code/ecdsap256/Hacl.Impl.ECDSA.MM.Exponent.fst
@@ -12,6 +12,7 @@ open FStar.Math.Lemmas
 open Hacl.Impl.P256.Math 
 
 open Hacl.Impl.P256.LowLevel 
+open Spec.P256.Lemmas
 open FStar.Tactics
 open FStar.Tactics.Canon 
 
