code/ecdsap256/Hacl.Impl.ECDSA.MM.Exponent.fsti
@@ -14,7 +14,6 @@ open Spec.P256.Lemmas
 open Spec.ECDSAP256.Definition
 open Spec.ECDSA
 open Hacl.Impl.P256.LowLevel 
-open Spec.P256.Ladder
 
 open Spec.P256.Lemmas
 
