code/ecdsap256/Hacl.Impl.P256.Core.fsti
@@ -16,7 +16,6 @@ open Spec.P256.Definitions
 open Spec.P256.SolinasReduction
 open Spec.P256.MontgomeryMultiplication
 open Spec.P256.MontgomeryMultiplication.PointAdd
-open Spec.P256.Ladder
 
 open Spec.P256
 
