Makefile
@@ -29,7 +29,7 @@
 # - vale-verify: properly staged target for re-verifying all the vale files
 # - vale-asm: re-generation of the Vale assemblies in dist/vale
 # - hacl-verify: staged target for verifying HACL* files
-#   curve25519-verify poly1305-verify chacha20-verify spec-verifyec
+#   curve25519-verify poly1305-verify chacha20-verify spec-verify
 #   code-verify: subsets of hacl-verify (each staged)
 #
 # To generate a Makefile for the interactive mode, use:
@@ -63,10 +63,10 @@ ifeq (,$(wildcard $(VALE_HOME)/bin/vale.exe))
   $(error $$VALE_HOME/bin/vale.exe does not exist$(newline)(VALE_HOME=$(VALE_HOME)).$(newline)Hint: ./tools/get_vale.sh if you don't have Vale, yet)
 endif
 
-# ifneq ($(shell cat $(VALE_HOME)/bin/.vale_version | tr -d '\r'),$(shell cat vale/.vale_version | tr -d '\r'))
-#   $(error this repository wants Vale $(shell cat vale/.vale_version) but in \
-#     $$VALE_HOME I found $(shell cat $(VALE_HOME)/bin/.vale_version).$(newline)(VALE_HOME=$(VALE_HOME))$(newline)Hint: ./tools/get_vale.sh)
-# endif
+ifneq ($(shell cat $(VALE_HOME)/bin/.vale_version | tr -d '\r'),$(shell cat vale/.vale_version | tr -d '\r'))
+  $(error this repository wants Vale $(shell cat vale/.vale_version) but in \
+    $$VALE_HOME I found $(shell cat $(VALE_HOME)/bin/.vale_version).$(newline)(VALE_HOME=$(VALE_HOME))$(newline)Hint: ./tools/get_vale.sh)
+endif
 
 endif
 endif
@@ -77,9 +77,9 @@ OPENSSL_HOME 	:= $(MLCRYPTO_HOME)/openssl
 endif
 
 ifeq (,$(NOOPENSSLCHECK))
-# ifeq (,$(OPENSSL_HOME))
-#   $(error Please define MLCRYPTO_HOME, possibly using cygpath -m on Windows)
-# endif
+ifeq (,$(OPENSSL_HOME))
+  $(error Please define MLCRYPTO_HOME, possibly using cygpath -m on Windows)
+endif
 
 ifeq (,$(OPENSSL_HOME)/libcrypto.a)
   $(error $$OPENSSL_HOME/libcrypto.a does not exist (OPENSSL_HOME=$(OPENSSL_HOME)))
@@ -669,13 +669,13 @@ BUNDLE_FLAGS	=\
   $(SALSA20_BUNDLE) \
   $(CURVE_BUNDLE) \
   $(CHACHAPOLY_BUNDLE) \
-  $(P256_BUNDLE) \
   $(ED_BUNDLE) \
   $(POLY_BUNDLE) \
   $(NACLBOX_BUNDLE) \
   $(MERKLE_BUNDLE) \
   $(WASMSUPPORT_BUNDLE) \
   $(CTR_BUNDLE) \
+  $(P256_BUNDLE) \
   $(FRODO_BUNDLE) \
   $(HPKE_BUNDLE) \
   $(STREAMING_BUNDLE) \
@@ -927,7 +927,7 @@ dist/mozilla/Makefile.basic: BLAKE2_BUNDLE = -bundle Hacl.Impl.Blake2.*,Hacl.Bla
 dist/mozilla/Makefile.basic: SHA3_BUNDLE = -bundle Hacl.SHA3
 dist/mozilla/Makefile.basic: HASH_BUNDLE = -bundle Hacl.Hash.*,Hacl.HKDF,Hacl.HMAC,Hacl.HMAC_DRBG
 dist/mozilla/Makefile.basic: HPKE_BUNDLE = -bundle 'Hacl.HPKE.*'
-dist/mozilla/Makefile.basic: P256_BUNDLE =
+dist/mozilla/Makefile.basic: ECDSA_BUNDLE =
 dist/mozilla/Makefile.basic: STREAMING_BUNDLE = -bundle Hacl.Streaming.*
 dist/mozilla/Makefile.basic: FRODO_BUNDLE = -bundle Hacl.Frodo.*,Hacl.SHA3,Hacl.Keccak,Frodo.Params
 dist/mozilla/Makefile.basic: \
